append_to_ancestor_list - 이 정도로 강력한 assume 도 안 통한다고...?

src/study/Nemonuri.Study.CSharpSyntaxRewriter2.Modifier2/Nemonuri.StratifiedNodes.Children.fst
@@ -10,12 +10,34 @@ let is_child #t (parent_node:N.node t) (node:N.node t)
   =
   N.lemma_node_level_is_greater_than_levels_of_nodes_in_children t;
   L.contains node (N.get_children parent_node)
+
+let rec skip_while #t 
+  (node_list:N.node_list t) 
+  (predicate:N.node t -> Tot bool)
+  : Tot (N.node_list t) (decreases node_list) =
+  match node_list with
+  | [] -> []
+  | hd::tl ->
+    match (predicate hd) with
+    | true -> node_list
+    | false -> skip_while tl predicate
 //---|
 
 //--- asserts ---
 let test_is_child1 = assert (
   forall (t:eqtype) (parent_node:N.node t) (node:N.node t).
     (is_child parent_node node) ==> (parent_node.level > node.level))
+//---|
+
+//--- propositions ---
+let node_list_is_ancestor_list #t (node_list:N.node_list t) : prop =
+  forall (n:N.node t).
+  let skipped = skip_while node_list (Prims.op_Equality n) in (
+    (L.length skipped >= 2) ==> (
+      let hd::tl = skipped in
+      is_child hd (L.hd tl)
+    )
+  )
 //---|
 
 //--- type definitions ---
@@ -27,6 +49,29 @@ let parent_child_selector (t:eqtype) (t2:Type) =
 let child_selector t (t2:Type) (parent:N.node t) =
   (child:N.node t{is_child parent child}) ->
   Tot t2
+
+let ancestor_list (t:eqtype) = 
+  al:(N.node_list t){ node_list_is_ancestor_list al }
+
+let can_append_to_ancestor_list #t (ancestor_list1:ancestor_list t) (ancestor_list2:ancestor_list t) //(node:N.node t)
+  : Tot bool =
+  match (ancestor_list1, ancestor_list2) with
+  | (hd1::tl1, hd2::tl2) -> is_child (L.last ancestor_list1) hd2
+  | _ -> true
+
+  //if (L.isEmpty al) then true
+  //else is_child (L.last al) node
+
+(*
+let rec append_to_ancestor_list #t (ancestor_list1:ancestor_list t) (ancestor_list2:ancestor_list t{ can_append_to_ancestor_list ancestor_list1 ancestor_list2 })
+  : Tot (ancestor_list t) (decreases ancestor_list1) =
+  match ancestor_list1 with
+  | [] -> ancestor_list2
+  | hd::tl -> (
+    assume ( forall (t:eqtype) (al:ancestor_list t). (not (L.isEmpty al)) ==> (node_list_is_ancestor_list (L.tl al)) );
+    hd::(append_to_ancestor_list tl ancestor_list2)
+  )
+*)
 //---|
 
 //--- theory members 2 ---
